Test/DafnyTests/TestAttribute.dfy
@@ -1,180 +1,175 @@
-// RUN: %dafny /compileVerbose:1 /compile:0 /spillTargetCode:3 /noVerify "%s" > "%t"
-// RUN: dotnet test -v:q -noLogo %S 2> %t.testresults.raw || true
-// Remove the timestamp prefixes on the expected errors
-// RUN: sed 's/[^]]*\]//' "%t".testresults.raw >> "%t"
-// RUN: %diff "%s.expect" "%t"
+// RUN: %dafny /verifyAllModules /compileVerbose:1 /compile:2 /spillTargetCode:1 /compileTarget:java /noVerify "%s" > "%t"
+
 
 include "../exceptions/VoidOutcomeDt.dfy"
 include "../exceptions/NatOutcomeDt.dfy"
 
-function method SafeDivide(a: nat, b: nat): NatOutcome {
-  if b == 0 then
-    NatFailure("Divide by zero")
-  else
-    NatSuccess(a/b)
-}
-
-method UnsafeDivide(a: nat, b: nat) returns (r: nat) {
-  expect b != 0;
-  return a/b;
-}
-
-method FailUnless(p: bool) returns (r: VoidOutcome) ensures r.VoidSuccess? ==> p {
-  if p {
-    return VoidSuccess;
-  } else {
-    return VoidFailure("requirement failed");
+module Div {
+  datatype VoidOutcome =
+  | VoidSuccess
+  | VoidFailure(error: string)
+  {
+      predicate method IsFailure() {
+          this.VoidFailure?
+      }
+      function method PropagateFailure(): VoidOutcome requires IsFailure() {
+          this
+      }
   }
-}
 
-function method {:test} PassingTest(): VoidOutcome {
-  VoidSuccess
-}
+  datatype NatOutcome =
+  | NatSuccess(value: nat)
+  | NatFailure(error: string)
+  {
+      predicate method IsFailure() {
+          this.NatFailure?
+      }
+      function method PropagateFailure(): NatOutcome requires IsFailure() {
+          this
+      }
+      function method Extract(): nat requires !IsFailure() {
+          this.value
+      }
+  }
 
-function method {:test} FailingTest(): VoidOutcome {
-  VoidFailure("Whoopsie")
-}
+  class Even {
+      var value:int;
+      function method IsValid():bool reads this {
+          this.value % 2 == 0
+      }
+      constructor (value:int) 
+          requires value % 2 == 0
+          ensures this.IsValid()
+      {
+          this.value := value;
+      }
+      function method Sum(a:int, b:int):int {
+          a + b
+      }
+  }
 
-method {:test} PassingTestUsingExpect() {
-  expect 2 + 2 == 4;
-}
+  class Divide {
 
-method {:test} FailingTestUsingExpect() {
-  expect 2 + 2 == 5;
-}
-
-method {:test} FailingTestUsingExpectWithMessage() {
-  expect 2 + 2 == 5, "Down with DoubleThink!";
-}
-
-method {:test} PassingTestUsingAssignOrHalt() {
-  var x := 5;
-  var y := 2;
-  var q :- expect SafeDivide(x, y);
-  expect q == 2;
-}
-
-method {:test} FailingTestUsingAssignOrHalt() {
-  var x := 5;
-  var y := 0;
-  var q :- expect SafeDivide(x, y);
-}
-
-method {:test} PassingTestUsingNoLHSAssignOrHalt() {
-  :- expect FailUnless(true);
-}
-
-method {:test} FailingTestUsingNoLHSAssignOrHalt() {
-  :- expect FailUnless(false);
-}
-
-class Even {
-    var value:int;
-    function method IsValid():bool reads this {
-        this.value % 2 == 0
+    function method SafeDivide(a: nat, b: nat): NatOutcome {
+      if b == 0 then
+        NatFailure("Divide by zero")
+      else
+        NatSuccess(a/b)
     }
-    constructor (value:int) 
-        requires value % 2 == 0
-        ensures this.IsValid()
-    {
-        this.value := value;
+
+    method UnsafeDivide(a: nat, b: nat) returns (r: nat) {
+      expect b != 0;
+      return a/b;
     }
-    function method Sum(a:int, b:int):int {
-        a + b
+
+    method FailUnless(p: bool) returns (r: VoidOutcome) ensures r.VoidSuccess? ==> p {
+      if p {
+        return VoidSuccess;
+      } else {
+        return VoidFailure("requirement failed");
+      }
     }
-}
 
-method {:extern} {:fresh} freshEven() returns (e:Even) ensures fresh(e)
+    function method {:test} PassingTest(): VoidOutcome {
+      VoidSuccess
+    }
 
-method {:test} PassingTestUsingFresh() {
-    var e:Even := freshEven();
-    e.value := 4;
-    expect(e.IsValid());
-}
+    function method {:test} FailingTest(): VoidOutcome {
+      VoidFailure("Whoopsie")
+    }
 
-method {:test} FailingTestUsingFresh() {
-    var e:Even := freshEven();
-    e.value := 5;
-    expect(e.IsValid());
-}
+    method {:test} PassingTestUsingExpect() {
+      expect 2 + 2 == 4;
+    }
 
-method {:extern} {:mock} MockValidEven() returns (e:Even) 
-    ensures fresh(e) 
-    ensures e.IsValid() == true
-method {:extern} {:mock} MockInValidEven() returns (e:Even) 
-    ensures fresh(e) 
-    ensures e.IsValid() == false
+    method {:test} FailingTestUsingExpect() {
+      expect 2 + 2 == 5;
+    }
 
-method {:test} PassingTestUsingValidMock() {
-    var e:Even := MockValidEven();
-    expect(e.IsValid());
-}
+    method {:test} FailingTestUsingExpectWithMessage() {
+      expect 2 + 2 == 5, "Down with DoubleThink!";
+    }
 
-method {:test} PassingTestUsingInValidMock() {
-    var e:Even := MockInValidEven();
-    expect(!e.IsValid());
-}
+    method {:test} PassingTestUsingAssignOrHalt() {
+      var x := 5;
+      var y := 2;
+      var q :- expect SafeDivide(x, y);
+      expect q == 2;
+    }
 
-method {:extern} {:mock} MockSum() returns (e:Even) 
-    ensures fresh(e) 
-    ensures e.Sum(2, 2) == 3
+    method {:test} FailingTestUsingAssignOrHalt() {
+      var x := 5;
+      var y := 0;
+      var q :- expect SafeDivide(x, y);
+    }
 
-method {:test} PassingMockSum() {
-    var e:Even := MockSum();
-    expect(e.Sum(2, 2) == 3);
-}
+    method {:test} PassingTestUsingNoLHSAssignOrHalt() {
+      :- expect FailUnless(true);
+    }
 
-method {:extern} {:mock} MockSumForall() returns (e:Even) 
-    ensures fresh(e) 
-    ensures forall a:int, b:int :: e.Sum(a, b) == 3
+    method {:test} FailingTestUsingNoLHSAssignOrHalt() {
+      :- expect FailUnless(false);
+    }
 
-method {:test} PassingMockForall() {
-    var e:Even := MockSumForall();
-    expect(e.Sum(2, 2) == 3);
-    expect(e.Sum(3, 2) == 3);
-}
+    method {:extern} {:fresh} freshEven() returns (e:Even) ensures fresh(e)
 
-method {:extern} {:mock} MockSumAsMultiplication() returns (e:Even) 
-    ensures fresh(e) 
-    ensures forall a:int, b:int :: e.Sum(a, b) == a * b
-    
-method {:test} PassingMockSumAsMultiplication() {
-    var e:Even := MockSumAsMultiplication();
-    expect(e.Sum(2, 2) == 4);
-    expect(e.Sum(2, 3) == 6);
-    expect(e.Sum(4, 0) == 0);
-    expect(e.Sum(5, 1) == 5);
-}
+    method {:test} PassingTestUsingFresh() {
+        var e:Even := freshEven();
+        e.value := 4;
+        expect(e.IsValid());
+    }
 
-method {:extern} {:mock} MockSumWithArgumentMatcher() returns (e:Even) 
-    ensures fresh(e) 
-    ensures forall a:int, b:int :: (a > b) ==> (e.Sum(a, b) == a * b)
-    ensures forall a:int, b:int :: (a <= b) ==> (e.Sum(a, b) == -a * b)
-    
-method {:test} PassingMockSumWithArgumentMatcher() {
-    var e:Even := MockSumWithArgumentMatcher();
-    expect(e.Sum(2, 2) == -4);
-    expect(e.Sum(2, 3) == -6);
-    expect(e.Sum(4, 0) == 0);
-    expect(e.Sum(5, 1) == 5);
-}
+    method {:test} FailingTestUsingFresh() {
+        var e:Even := freshEven();
+        e.value := 5;
+        expect(e.IsValid());
+    }
 
-method {:extern} {:mock} MockField() returns (e:Even) 
-    ensures fresh(e) 
-    ensures e.value == 7;
-    
-method {:test} PassingMockField() {
-    var e:Even := MockField();
-    expect(e.value == 7);
-    expect(e.value != 5);
-}
+    method {:extern} {:mock} MockValidEven() returns (e:Even) 
+        ensures fresh(e) 
+        ensures e.IsValid() == true
 
-method {:extern} {:mock} ParametrizedMock(a: int) returns (e:Even) 
-    ensures fresh(e) 
-    ensures e.value == a;
-    
-method {:test} PassingParameterizedMock() {
-    var e:Even := ParametrizedMock(24);
-    expect(e.value == 24);
-    expect(e.value != 7);
+    method {:extern} {:mock} MockInValidEven() returns (e:Even) 
+        ensures fresh(e) 
+        ensures e.IsValid() == false
+
+    method {:test} PassingTestUsingValidMock() {
+        var e:Even := MockValidEven();
+        expect(e.IsValid());
+    }
+
+    method {:test} PassingTestUsingInValidMock() {
+        var e:Even := MockInValidEven();
+        expect(!e.IsValid());
+    }
+
+    method {:extern} {:mock} MockSum() returns (e:Even) 
+        ensures fresh(e) 
+        ensures e.Sum(2, 2) == 3
+
+    method {:test} PassingMockSum() {
+        var e:Even := MockSum();
+        expect(e.Sum(2, 2) == 3);
+    }
+
+    method {:extern} {:mock} MockField() returns (e:Even) 
+        ensures fresh(e) 
+        ensures e.value == 7;
+        
+    method {:test} PassingMockField() {
+        var e:Even := MockField();
+        expect(e.value == 7);
+        expect(e.value != 5);
+    }
+
+    method {:extern} {:mock} ParametrizedMock(a: int) returns (e:Even) 
+        ensures fresh(e) 
+        ensures e.value == a;
+        
+    method {:test} PassingParameterizedMock() {
+        var e:Even := ParametrizedMock(24);
+        expect(e.value == 24);
+        expect(e.value != 7);
+    }
+  }
 }
